demo/test_proof.v
@@ -19,7 +19,25 @@ Qed.
 Definition Any {A:Type} (X:unit) (x:A) := [].
 
 Definition Myrecord _A _B A B C (TA:htype A _A) (TB:htype B int) (TC:htype C val) X Y Z (l:loc) :=
-  Hexists (x:_A) (y:int) (z:val), (l ~~> @_myrecord_of _A _B x y z) \* TA X x \* TB Y y \* TC Z z.
+  Hexists (x:_A) (y:int) (z:val), heap_is_single l (@_myrecord_of _A _B x y z) \* TA X x \* TB Y y \* TC Z z.
+
+Lemma Myrecord_focus: forall _A _B A B C (TA:htype A _A) (TB:htype B int) (TC:htype C val) X Y Z (l:loc),
+   l ~> Myrecord _B TA TB TC X Y Z ==>
+  Hexists (x:_A) (y:int) (z:val),
+  l ~> Myrecord _B Id Id Id x y z \* TA X x \* TB Y y \* TC Z z.
+Proof.
+  intros. unfold Myrecord at 1. hdata_simpl. hextract.
+  unfold Myrecord at 1. hsimpl. hdata_simpl. hsimpl~.
+Qed.
+
+Lemma Myrecord_unfocus: forall _A _B A B C (TA:htype A _A) (TB:htype B int) (TC:htype C val) X Y Z (l:loc), 
+  forall (x:_A) (y:int) (z:val),
+  l ~> Myrecord _B Id Id Id x y z \* TA X x \* TB Y y \* TC Z z ==>
+   l ~> Myrecord _B TA TB TC X Y Z.
+Proof.
+  intros. unfold Myrecord at 1. hdata_simpl. hextract.
+  unfold Myrecord at 1. hdata_simpl. subst. hsimpl~.
+Qed.
 
 Parameter _get_rectwo_spec : forall _A _B (A C:Type),
   Spec _get_rectwo (l:loc) |R>> forall (TA:htype A _A) (TC:htype C val) X Y Z,
